add missing func. WIP: allocate_slab_aux_2

src/Slabs.fst
@@ -953,7 +953,97 @@ let allocate_slab_aux_1
     return r
   )
 
-assume val allocate_slab_aux_2
+#push-options "--z3rlimit 75 --compat_pre_typed_indexed_effects"
+assume val allocate_slab_aux_2_full
+  (size_class: sc)
+  (slab_region: array U8.t{A.length slab_region = U32.v metadata_max * U32.v page_size})
+  (md_bm_region: array U64.t{A.length md_bm_region = U32.v metadata_max * 4})
+  (md_region: array AL.cell{A.length md_region = U32.v metadata_max})
+  (md_count: ref U32.t)
+  (r1 r2 r3: ref US.t)
+  (md_count_v: U32.t{U32.v md_count_v <= U32.v metadata_max})
+  (md_region_lv: G.erased (Seq.lseq AL.status (U32.v md_count_v)))
+  (idx1: US.t)
+  (idx2: US.t{US.v idx2 < U32.v md_count_v})
+  (idx3: US.t)
+  //: Steel (array U8.t)
+  : Steel unit
+  (
+    vptr md_count `star`
+    vptr r1 `star`
+    vptr r2 `star`
+    vptr r3 `star`
+    (AL.varraylist pred1 pred2 pred3
+      (A.split_l md_region (u32_to_sz md_count_v))
+      (US.v idx1) (US.v idx2) (US.v idx3)) `star`
+    starseq
+      #(pos:U32.t{U32.v pos < U32.v md_count_v})
+      #(t size_class)
+      (f size_class slab_region md_bm_region md_count_v (Seq.upd (G.reveal md_region_lv) (US.v idx2) 2ul))
+      (f_lemma size_class slab_region md_bm_region md_count_v (Seq.upd (G.reveal md_region_lv) (US.v idx2) 2ul))
+      (SeqUtils.init_u32_refined (U32.v md_count_v))
+  )
+  (fun _ ->
+    vrefinedep
+      (vptr md_count)
+      (fun x -> U32.v x <= U32.v metadata_max == true)
+      (fun v -> left_vprop size_class slab_region md_bm_region v md_region r1 r2 r3)
+  )
+  (requires fun h0 ->
+    sel md_count h0 == md_count_v /\
+    sel r1 h0 == idx1 /\
+    sel r2 h0 == idx2 /\
+    sel r3 h0 == idx3 /\
+    idx2 <> AL.null_ptr
+  )
+  (ensures fun _ _ _ -> True)
+
+
+assume val allocate_slab_aux_2_partial
+  (size_class: sc)
+  (slab_region: array U8.t{A.length slab_region = U32.v metadata_max * U32.v page_size})
+  (md_bm_region: array U64.t{A.length md_bm_region = U32.v metadata_max * 4})
+  (md_region: array AL.cell{A.length md_region = U32.v metadata_max})
+  (md_count: ref U32.t)
+  (r1 r2 r3: ref US.t)
+  (md_count_v: U32.t{U32.v md_count_v <= U32.v metadata_max})
+  (md_region_lv: G.erased (Seq.lseq AL.status (U32.v md_count_v)))
+  (idx1: US.t)
+  (idx2: US.t{US.v idx2 < U32.v md_count_v})
+  (idx3: US.t)
+  //: Steel (array U8.t)
+  : Steel unit
+  (
+    vptr md_count `star`
+    vptr r1 `star`
+    vptr r2 `star`
+    vptr r3 `star`
+    (AL.varraylist pred1 pred2 pred3
+      (A.split_l md_region (u32_to_sz md_count_v))
+      (US.v idx1) (US.v idx2) (US.v idx3)) `star`
+    starseq
+      #(pos:U32.t{U32.v pos < U32.v md_count_v})
+      #(t size_class)
+      (f size_class slab_region md_bm_region md_count_v (G.reveal md_region_lv))
+      (f_lemma size_class slab_region md_bm_region md_count_v (G.reveal md_region_lv))
+      (SeqUtils.init_u32_refined (U32.v md_count_v))
+  )
+  (fun _ ->
+    vrefinedep
+      (vptr md_count)
+      (fun x -> U32.v x <= U32.v metadata_max == true)
+      (fun v -> left_vprop size_class slab_region md_bm_region v md_region r1 r2 r3)
+  )
+  (requires fun h0 ->
+    sel md_count h0 == md_count_v /\
+    sel r1 h0 == idx1 /\
+    sel r2 h0 == idx2 /\
+    sel r3 h0 == idx3 /\
+    idx2 <> AL.null_ptr
+  )
+  (ensures fun _ _ _ -> True)
+
+let allocate_slab_aux_2
   (size_class: sc)
   (slab_region: array U8.t{A.length slab_region = U32.v metadata_max * U32.v page_size})
   (md_bm_region: array U64.t{A.length md_bm_region = U32.v metadata_max * 4})
@@ -1001,6 +1091,214 @@ assume val allocate_slab_aux_2
       (fun v -> left_vprop size_class slab_region md_bm_region v md_region r1 r2 r3)
     ) in
     md_count_v == dfst blob1)
+  =
+  let idx2' : US.t = read r2 in
+  change_equal_slprop
+    (AL.varraylist pred1 pred2 pred3
+      (A.split_l md_region (u32_to_sz md_count_v))
+      (US.v idx1) (US.v idx2) (US.v idx3))
+    (AL.varraylist pred1 pred2 pred3
+      (A.split_l md_region (u32_to_sz md_count_v))
+      (US.v idx1) (US.v idx2') (US.v idx3));
+  //TODO @Aymeric: here idx1' == idx1,
+  //deduce heads are < len of the varraylist
+  assume (US.v idx2' < U32.v md_count_v);
+  starseq_unpack_s
+    #_
+    #(pos:U32.t{U32.v pos < U32.v md_count_v})
+    #(t size_class)
+    (f size_class slab_region md_bm_region md_count_v md_region_lv)
+    (f_lemma size_class slab_region md_bm_region md_count_v md_region_lv)
+    (SeqUtils.init_u32_refined (U32.v md_count_v))
+    (US.v idx2');
+  //TODO @Aymeric: x \in dlist hd1 ==> pred1 x
+  assume (Seq.index md_region_lv (US.v idx2') == 0ul);
+  SeqUtils.init_u32_refined_index (U32.v md_count_v) (US.v idx2');
+  change_slprop_rel
+     (f size_class slab_region md_bm_region md_count_v md_region_lv (Seq.index (SeqUtils.init_u32_refined (U32.v md_count_v)) (US.v idx2')))
+     (p_partial size_class (md_bm_array md_bm_region (US.sizet_to_uint32 idx2'), slab_array slab_region (US.sizet_to_uint32 idx2')))
+     (fun x y -> x == y)
+     (fun _ -> admit ());
+  p_partial_unpack size_class
+     (md_bm_array md_bm_region (US.sizet_to_uint32 idx2'), slab_array slab_region (US.sizet_to_uint32 idx2'))
+     (md_bm_array md_bm_region (US.sizet_to_uint32 idx2'), slab_array slab_region (US.sizet_to_uint32 idx2'));
+  let r = allocate_slot size_class
+    (md_bm_array md_bm_region (US.sizet_to_uint32 idx2'))
+    (slab_array slab_region (US.sizet_to_uint32 idx2'))
+  in
+  let cond = allocate_slab_aux_cond size_class
+    (md_bm_array md_bm_region (US.sizet_to_uint32 idx2'))
+    (slab_array slab_region (US.sizet_to_uint32 idx2'))
+  in
+  if cond then (
+   change_slprop_rel
+      (slab_vprop size_class
+        (slab_array slab_region (US.sizet_to_uint32 idx2'))
+        (md_bm_array md_bm_region (US.sizet_to_uint32 idx2')))
+      (f size_class slab_region md_bm_region md_count_v
+        (Seq.upd md_region_lv (US.v idx2') 2ul)
+        (Seq.index (SeqUtils.init_u32_refined (U32.v md_count_v)) (US.v idx2')))
+      (fun x y -> x == y)
+      (fun _ -> admit ());
+    //TODO: starseq aux lemma
+    admit ();
+    starseq_upd_pack
+      #_
+      #(pos:U32.t{U32.v pos < U32.v md_count_v})
+      #(t size_class)
+      (f size_class slab_region md_bm_region md_count_v md_region_lv)
+      (f size_class slab_region md_bm_region md_count_v (Seq.upd (G.reveal md_region_lv) (US.v idx2') 2ul))
+      (f_lemma size_class slab_region md_bm_region md_count_v md_region_lv)
+      (f_lemma size_class slab_region md_bm_region md_count_v (Seq.upd (G.reveal md_region_lv) (US.v idx2') 2ul))
+      (SeqUtils.init_u32_refined (U32.v md_count_v))
+      (SeqUtils.init_u32_refined (U32.v md_count_v))
+      (US.v idx2');
+    allocate_slab_aux_2_full
+      size_class
+      slab_region
+      md_bm_region
+      md_region
+      md_count
+      r1 r2 r3
+      md_count_v
+      md_region_lv
+      idx1 idx2' idx3;
+    return r
+) else (
+  admit ();
+  change_slprop_rel
+      (slab_vprop size_class
+        (slab_array slab_region (US.sizet_to_uint32 idx2'))
+        (md_bm_array md_bm_region (US.sizet_to_uint32 idx2')))
+      (f size_class slab_region md_bm_region md_count_v (G.reveal md_region_lv)
+        (Seq.index (SeqUtils.init_u32_refined (U32.v md_count_v)) (US.v idx2')))
+      (fun x y -> x == y)
+      (fun _ -> admit ());
+    starseq_pack_s
+      #_
+      #(pos:U32.t{U32.v pos < U32.v md_count_v})
+      #(t size_class)
+      (f size_class slab_region md_bm_region md_count_v md_region_lv)
+      (f_lemma size_class slab_region md_bm_region md_count_v md_region_lv)
+      (SeqUtils.init_u32_refined (U32.v md_count_v))
+      (US.v idx2');
+    allocate_slab_aux_2_partial
+      size_class
+      slab_region
+      md_bm_region
+      md_region
+      md_count
+      r1 r2 r3
+      md_count_v
+      md_region_lv
+      idx1 idx2' idx3;
+    return r
+  )
+
+let allocate_slab_aux_2_full
+  (size_class: sc)
+  (slab_region: array U8.t{A.length slab_region = U32.v metadata_max * U32.v page_size})
+  (md_bm_region: array U64.t{A.length md_bm_region = U32.v metadata_max * 4})
+  (md_region: array AL.cell{A.length md_region = U32.v metadata_max})
+  (md_count: ref U32.t)
+  (r1 r2 r3: ref US.t)
+  (md_count_v: U32.t{U32.v md_count_v <= U32.v metadata_max})
+  (md_region_lv: G.erased (Seq.lseq AL.status (U32.v md_count_v)))
+  (idx1: US.t)
+  (idx2: US.t{US.v idx2 < U32.v md_count_v})
+  (idx3: US.t)
+  //: Steel (array U8.t)
+  : Steel unit
+  (
+    vptr md_count `star`
+    vptr r1 `star`
+    vptr r2 `star`
+    vptr r3 `star`
+    (AL.varraylist pred1 pred2 pred3
+      (A.split_l md_region (u32_to_sz md_count_v))
+      (US.v idx1) (US.v idx2) (US.v idx3)) `star`
+    starseq
+      #(pos:U32.t{U32.v pos < U32.v md_count_v})
+      #(t size_class)
+      (f size_class slab_region md_bm_region md_count_v (Seq.upd (G.reveal md_region_lv) (US.v idx2) 2ul))
+      (f_lemma size_class slab_region md_bm_region md_count_v (Seq.upd (G.reveal md_region_lv) (US.v idx2) 2ul))
+      (SeqUtils.init_u32_refined (U32.v md_count_v))
+  )
+  (fun _ ->
+    vrefinedep
+      (vptr md_count)
+      (fun x -> U32.v x <= U32.v metadata_max == true)
+      (fun v -> left_vprop size_class slab_region md_bm_region v md_region r1 r2 r3)
+  )
+  (requires fun h0 ->
+    sel md_count h0 == md_count_v /\
+    sel r1 h0 == idx1 /\
+    sel r2 h0 == idx2 /\
+    sel r3 h0 == idx3 /\
+    idx2 <> AL.null_ptr
+  )
+  (ensures fun _ _ _ -> True)
+  =
+  //assume (t_of (
+  //  AL.varraylist pred1 pred2 pred3
+  //    (A.split_l md_region (u32_to_sz md_count))
+  //    (US.v idx1) (US.v idx2) (US.v idx3))
+  //  ==
+  //  v:Seq.seq (AL.cell status){AL.varraylist_refine pred1 pred2 pred3 (US.v idx1) (US.v idx2) (US.v idx3) v});
+  //let l
+  //  = gget (
+  //  AL.varraylist pred1 pred2 pred3
+  //    (A.split_l md_region (u32_to_sz md_count))
+  //    (US.v idx1) (US.v idx2) (US.v idx3)
+  //) in
+  //TODO @Aymeric: deduce mem x x::_
+  //assume (AL.mem (US.v idx1) (US.v idx1) (G.reveal l));
+  admit ();
+  let idx2' = AL.remove1 #pred1 #pred2 #pred3
+    (A.split_l md_region (u32_to_sz md_count_v))
+    idx1 (Ghost.hide (US.v idx2)) (Ghost.hide (US.v idx3)) idx1 in
+  //TODO @Aymeric: refine insert3 spec
+  AL.insert3 #pred1 #pred2 #pred3
+    (A.split_l md_region (u32_to_sz md_count_v))
+    idx3 (Ghost.hide (US.v idx1')) (Ghost.hide (US.v idx2)) idx1 2ul;
+  write r1 idx1';
+  write r3 idx1;
+  intro_vdep
+    (vptr r1 `star` vptr r2 `star` vptr r3)
+    (AL.varraylist pred1 pred2 pred3
+      (A.split_l md_region (u32_to_sz md_count_v))
+      (US.v idx1') (US.v idx2) (US.v idx1))
+    (fun (idxs: (US.t & US.t) & US.t) ->
+      AL.varraylist pred1 pred2 pred3
+        (A.split_l md_region (u32_to_sz md_count_v))
+
+      (US.v (fst (fst idxs)))
+      (US.v (snd (fst idxs)))
+      (US.v (snd idxs))
+    );
+  slassert (left_vprop1 md_region md_count_v r1 r2 r3);
+  slassert (left_vprop2 size_class slab_region md_bm_region md_count_v (Seq.upd (G.reveal md_region_lv) (US.v idx1) 2ul));
+  intro_vdep
+    (left_vprop1 md_region md_count_v r1 r2 r3)
+    (left_vprop2 size_class slab_region md_bm_region md_count_v
+      (Seq.upd (G.reveal md_region_lv) (US.v idx1) 2ul))
+
+    (fun x -> left_vprop2 size_class slab_region md_bm_region md_count_v (dataify (dsnd x)));
+  slassert (left_vprop size_class slab_region md_bm_region md_count_v md_region r1 r2 r3);
+  intro_vrefinedep
+    (vptr md_count)
+    (fun x -> U32.v x <= U32.v metadata_max == true)
+    (fun v -> left_vprop size_class slab_region md_bm_region v md_region r1 r2 r3)
+    (left_vprop size_class slab_region md_bm_region md_count_v md_region r1 r2 r3)
+
+
+
+
+
+
+
+(*)
+
 
 #push-options "--fuel 0 --ifuel 0"
 let empty_md_is_properly_zeroed
